implies classical

Foundation/ProvabilityLogic/Arithmetic.lean
@@ -13,8 +13,46 @@ open FirstOrder
 
 namespace Modal
 
+namespace Logic
+
 /-- `L` is provability logic of `T` relative to metatheory `U` -/
-def Logic.IsProvabilityLogic (L : Modal.Logic ℕ) (T U : ArithmeticTheory) [T.Δ₁] := ∀ A, L ⊢ A ↔ ∀ f : T.StandardRealization, U ⊢ f A
+def IsProvabilityLogic (L : Modal.Logic ℕ) (T U : ArithmeticTheory) [T.Δ₁] := ∀ A, L ⊢ A ↔ ∀ f : T.StandardRealization, U ⊢ f A
+
+variable {T U : ArithmeticTheory} [T.Δ₁] {L : Modal.Logic ℕ}
+
+/-- `L` is Łukasiewicz if `L` is provability logic. -/
+def inst_Łukasiewiicz_of_isProvabilityLogic (hPL : L.IsProvabilityLogic T U) : Entailment.Łukasiewicz L where
+  mdp := by
+    rintro A B ⟨hA⟩ ⟨hB⟩;
+    constructor;
+    simp only [←Modal.Logic.iff_provable, hPL A, hPL B, hPL (A ➝ B)] at hA hB ⊢;
+    intro f;
+    replace hA : U ⊢ f A ➝ f B := hA f;
+    replace hB : U ⊢ f A := hB f;
+    cl_prover [hA, hB];
+  implyK {_ _} := by
+    constructor;
+    apply Modal.Logic.iff_provable.mp;
+    apply hPL _ |>.mpr;
+    simp;
+  implyS {_ _ _} := by
+    constructor;
+    apply Modal.Logic.iff_provable.mp;
+    apply hPL _ |>.mpr;
+    simp;
+  elimContra {_ _} := by
+    constructor;
+    apply Modal.Logic.iff_provable.mp;
+    apply hPL _ |>.mpr;
+    intro f;
+    dsimp [ProvabilityLogic.Realization.interpret];
+    cl_prover;
+
+def inst_Cl_of_isProvabilityLogic (hPL : L.IsProvabilityLogic T U) : Entailment.Cl L := by
+  have := inst_Łukasiewiicz_of_isProvabilityLogic hPL;
+  infer_instance;
+
+end Logic
 
 end Modal
 
@@ -37,34 +75,7 @@ lemma isProvabilityLogic_provabilityLogicOn : (T.provabilityLogicOn U).IsProvabi
 lemma provabilityLogicOn.provable_iff : (T.provabilityLogicOn U) ⊢ A ↔ ∀ f : T.StandardRealization, U ⊢ f A := by
   simp [Modal.Logic.iff_provable, provabilityLogicOn]
 
-instance : Entailment.Łukasiewicz (T.provabilityLogicOn U) where
-  mdp := by
-    rintro A B ⟨hA⟩ ⟨hB⟩;
-    constructor;
-    simp only [←Modal.Logic.iff_provable, provabilityLogicOn.provable_iff] at hA hB ⊢;
-    intro f;
-    replace hA : U ⊢ f A ➝ f B := hA f;
-    replace hB : U ⊢ f A := hB f;
-    cl_prover [hA, hB];
-  implyK {_ _} := by
-    constructor;
-    apply Modal.Logic.iff_provable.mp;
-    apply provabilityLogicOn.provable_iff.mpr;
-    simp;
-  implyS {_ _ _} := by
-    constructor;
-    apply Modal.Logic.iff_provable.mp;
-    apply provabilityLogicOn.provable_iff.mpr;
-    simp;
-  elimContra {_ _} := by
-    constructor;
-    apply Modal.Logic.iff_provable.mp;
-    apply provabilityLogicOn.provable_iff.mpr;
-    intro f;
-    dsimp [ProvabilityLogic.Realization.interpret];
-    cl_prover;
-
-instance : Entailment.Cl (T.provabilityLogicOn U) where
+instance : Entailment.Cl (T.provabilityLogicOn U) := Modal.Logic.inst_Cl_of_isProvabilityLogic isProvabilityLogic_provabilityLogicOn
 
 end ArithmeticTheory
 
